code/ecdsap256/Hacl.Impl.P256.Scalar.fst
@@ -17,38 +17,25 @@ module SM = Hacl.Spec.P256.Montgomery
 
 module BD = Hacl.Spec.Bignum.Definitions
 module BM = Hacl.Bignum.Montgomery
-module SBM = Hacl.Spec.Bignum.Montgomery
-module SBML = Hacl.Spec.Montgomery.Lemmas
 
 friend Hacl.Bignum256
 
 #reset-options "--z3rlimit 50 --fuel 0 --ifuel 0"
 
-val qmod_short_lemma: a:nat{a < pow2 256} ->
-  Lemma (let r = if a >= S.order then a - S.order else a in r = a % S.order)
-
-let qmod_short_lemma a =
-  let r = if a >= S.order then a - S.order else a in
-  if a >= S.order then begin
-    Math.Lemmas.lemma_mod_sub a S.order 1;
-    assert_norm (pow2 256 - S.order < S.order);
-    Math.Lemmas.small_mod r S.order end
-  else
-   Math.Lemmas.small_mod r S.order
-
+///  Create one
 
 [@CInline]
-let qmod_short x res =
-  push_frame ();
-  let tmp = create_felem () in
-  make_order tmp;
-  let h0 = ST.get () in
-  let c = bn_sub4 tmp x tmp in
-  bn_cmovznz4 res c tmp x;
-  SB.as_nat_bound (as_seq h0 x);
-  qmod_short_lemma (as_nat h0 x);
-  pop_frame ()
+let make_qone n =
+  [@inline_let] let n0 = u64 0xc46353d039cdaaf in
+  [@inline_let] let n1 = u64 0x4319055258e8617b in
+  [@inline_let] let n2 = u64 0x0 in
+  [@inline_let] let n3 = u64 0xffffffff in
+  assert_norm (v n0 + v n1 * pow2 64 + v n2 * pow2 128 + v n3 * pow2 192 == SM.toDomain_ 1);
+  assert_norm (SM.fromDomain_ (v n0 + v n1 * pow2 64 + v n2 * pow2 128 + v n3 * pow2 192) == 1);
+  bn_make_u64_4 n n0 n1 n2 n3
 
+
+///  Comparison
 
 [@CInline]
 let bn_is_lt_order_mask4 f =
@@ -78,154 +65,45 @@ let bn_is_lt_order_and_gt_zero_mask4 f =
   res
 
 
-//----------------------
-// TODO: share the proofs with Hacl.Spec.P256.Montgomerymultiplication
+///  Field Arithmetic
 
-let lemmaFromDomain a = ()
+val qmod_short_lemma: a:nat{a < pow2 256} ->
+  Lemma (let r = if a >= S.order then a - S.order else a in r = a % S.order)
 
-let lemmaToDomain a = ()
-
-// toDomain_ (fromDomain_ a) == a
-let lemmaFromDomainToDomain a =
-  calc (==) {
-    toDomain_ (fromDomain_ a); // == a
-    (==) { }
-    (a * qmont_R_inv % S.order) * qmont_R % S.order;
-    (==) { Math.Lemmas.lemma_mod_mul_distr_l (a * qmont_R_inv) qmont_R S.order }
-    a * qmont_R_inv * qmont_R % S.order;
-    (==) { Math.Lemmas.paren_mul_right a qmont_R_inv qmont_R }
-    a * (qmont_R_inv * qmont_R) % S.order;
-    (==) { Math.Lemmas.lemma_mod_mul_distr_r a (qmont_R_inv * qmont_R) S.order }
-    a * (qmont_R_inv * qmont_R % S.order) % S.order;
-    (==) { assert_norm (qmont_R_inv * qmont_R % S.order = 1) }
-    a % S.order;
-    (==) { Math.Lemmas.modulo_lemma a S.order }
-    a;
-  }
+let qmod_short_lemma a =
+  let r = if a >= S.order then a - S.order else a in
+  if a >= S.order then begin
+    Math.Lemmas.lemma_mod_sub a S.order 1;
+    assert_norm (pow2 256 - S.order < S.order);
+    Math.Lemmas.small_mod r S.order end
+  else
+   Math.Lemmas.small_mod r S.order
 
 
-// fromDomain_ (toDomain_ a) == a
-let lemmaToDomainFromDomain a =
-  calc (==) {
-    fromDomain_ (toDomain_ a); // == a
-    (==) { }
-    (a * qmont_R % S.order) * qmont_R_inv % S.order;
-    (==) { Math.Lemmas.lemma_mod_mul_distr_l (a * qmont_R) qmont_R_inv S.order }
-    a * qmont_R * qmont_R_inv % S.order;
-    (==) { Math.Lemmas.paren_mul_right a qmont_R qmont_R_inv }
-    a * (qmont_R * qmont_R_inv) % S.order;
-    (==) { Math.Lemmas.lemma_mod_mul_distr_r a (qmont_R * qmont_R_inv) S.order }
-    a * (qmont_R * qmont_R_inv % S.order) % S.order;
-    (==) { assert_norm (qmont_R * qmont_R_inv % S.order = 1) }
-    a % S.order;
-    (==) { Math.Lemmas.modulo_lemma a S.order }
-    a;
-  }
+[@CInline]
+let qmod_short x res =
+  push_frame ();
+  let tmp = create_felem () in
+  make_order tmp;
+  let h0 = ST.get () in
+  let c = bn_sub4 tmp x tmp in
+  bn_cmovznz4 res c tmp x;
+  SB.as_nat_bound (as_seq h0 x);
+  qmod_short_lemma (as_nat h0 x);
+  pop_frame ()
 
 
-val qadd_lemma: a:S.qelem -> b:S.qelem ->
-  Lemma (S.qadd (fromDomain_ a) (fromDomain_ b) = fromDomain_ ((a + b) % S.order))
-
-let qadd_lemma a b =
-  calc (==) {
-    (fromDomain_ a + fromDomain_ b) % S.order;
-    (==) { }
-    (a * qmont_R_inv % S.order + b * qmont_R_inv % S.order) % S.order;
-    (==) { Math.Lemmas.modulo_distributivity (a * qmont_R_inv) (b * qmont_R_inv) S.order }
-    (a * qmont_R_inv + b * qmont_R_inv) % S.order;
-    (==) { Math.Lemmas.distributivity_add_left a b qmont_R_inv }
-    (a + b) * qmont_R_inv % S.order;
-    (==) { Math.Lemmas.lemma_mod_mul_distr_l (a + b) qmont_R_inv S.order }
-    (a + b) % S.order * qmont_R_inv % S.order;
-    (==) { }
-    fromDomain_ ((a + b) % S.order);
-  }
-
-
-val qmul_lemma: a:S.qelem -> b:S.qelem ->
-  Lemma (S.qmul (fromDomain_ a) (fromDomain_ b) = fromDomain_ ((a * b * qmont_R_inv) % S.order))
-
-let qmul_lemma a b =
-  calc (==) {
-    (fromDomain_ a * fromDomain_ b) % S.order;
-    (==) { }
-    ((a * qmont_R_inv % S.order) * (b * qmont_R_inv % S.order)) % S.order;
-    (==) { Math.Lemmas.lemma_mod_mul_distr_l
-      (a * qmont_R_inv) (b * qmont_R_inv % S.order) S.order }
-    (a * qmont_R_inv * (b * qmont_R_inv % S.order)) % S.order;
-    (==) { Math.Lemmas.lemma_mod_mul_distr_r (a * qmont_R_inv) (b * qmont_R_inv) S.order }
-    (a * qmont_R_inv * (b * qmont_R_inv)) % S.order;
-    (==) { Math.Lemmas.paren_mul_right a qmont_R_inv (b * qmont_R_inv) }
-    (a * (qmont_R_inv * (b * qmont_R_inv))) % S.order;
-    (==) { Math.Lemmas.paren_mul_right qmont_R_inv b qmont_R_inv }
-    (a * (qmont_R_inv * b * qmont_R_inv)) % S.order;
-    (==) { Math.Lemmas.swap_mul qmont_R_inv b }
-    (a * (b * qmont_R_inv * qmont_R_inv)) % S.order;
-    (==) { Math.Lemmas.paren_mul_right a (b * qmont_R_inv) qmont_R_inv }
-    (a * (b * qmont_R_inv) * qmont_R_inv) % S.order;
-    (==) { Math.Lemmas.paren_mul_right a b qmont_R_inv }
-    (a * b * qmont_R_inv * qmont_R_inv) % S.order;
-    (==) { Math.Lemmas.lemma_mod_mul_distr_l (a * b * qmont_R_inv) qmont_R_inv S.order }
-    fromDomain_ ((a * b * qmont_R_inv) % S.order);
-  }
-
-//---------------------
-
-val qmont_R_inv_is_bn_mont_d: unit -> Lemma
-  (requires S.order % 2 = 1)
-  (ensures  (let d, _ = SBML.eea_pow2_odd 256 S.order in qmont_R_inv == d % S.order))
-
-let qmont_R_inv_is_bn_mont_d () =
-  let d, k = SBML.eea_pow2_odd 256 S.order in
-  SBML.mont_preconditions_d 64 4 S.order;
-  assert (d * pow2 256 % S.order = 1);
-
-  assert_norm (qmont_R * qmont_R_inv % S.order = 1);
-  Math.Lemmas.lemma_mod_mul_distr_l (pow2 256) qmont_R_inv S.order;
-  assert (qmont_R_inv * pow2 256 % S.order = 1);
-
-  assert (qmont_R_inv * pow2 256 % S.order = d * pow2 256 % S.order);
-  SM.lemma_mod_mul_pow256_order qmont_R_inv d;
-  assert (qmont_R_inv % S.order == d % S.order);
-  Math.Lemmas.modulo_lemma qmont_R_inv S.order;
-  assert (qmont_R_inv == d % S.order)
-
-
-val lemma_order_mont: unit ->
-  Lemma (S.order % 2 = 1 /\ S.order < pow2 256 /\ (1 + S.order * 0xccd1c8aaee00bc4f) % pow2 64 = 0)
-
-let lemma_order_mont () =
-  assert_norm (S.order % 2 = 1);
-  assert_norm (S.order < pow2 256);
-  assert_norm ((1 + S.order * 0xccd1c8aaee00bc4f) % pow2 64 = 0)
-
-
-val qmont_reduction_lemma: x:Lib.Sequence.lseq uint64 8 -> n:Lib.Sequence.lseq uint64 4 -> Lemma
-  (requires BD.bn_v n = S.order /\ BD.bn_v x < S.order * S.order)
-  (ensures  BD.bn_v (SBM.bn_mont_reduction n (u64 0xccd1c8aaee00bc4f) x) ==
-    BD.bn_v x * qmont_R_inv % S.order)
-
-let qmont_reduction_lemma x n =
-  let k0 = 0xccd1c8aaee00bc4f in
-  lemma_order_mont ();
-  assert (SBM.bn_mont_pre n (u64 k0));
-  let d, _ = SBML.eea_pow2_odd 256 (BD.bn_v n) in
-
-  let res = SBM.bn_mont_reduction n (u64 k0) x in
-  assert_norm (S.order * S.order < S.order * pow2 256);
-  assert (BD.bn_v x < S.order * pow2 256);
-
-  SBM.bn_mont_reduction_lemma n (u64 k0) x;
-  assert (BD.bn_v res == SBML.mont_reduction 64 4 (BD.bn_v n) k0 (BD.bn_v x));
-  SBML.mont_reduction_lemma 64 4 (BD.bn_v n) k0 (BD.bn_v x);
-  assert (BD.bn_v res == BD.bn_v x * d % S.order);
-  calc (==) {
-    (BD.bn_v x) * d % S.order;
-    (==) { Math.Lemmas.lemma_mod_mul_distr_r (BD.bn_v x) d S.order }
-    (BD.bn_v x) * (d % S.order) % S.order;
-    (==) { qmont_R_inv_is_bn_mont_d () }
-    (BD.bn_v x) * qmont_R_inv % S.order;
-  }
+[@CInline]
+let qadd x y res =
+  let h0 = ST.get () in
+  push_frame ();
+  let n = create_felem () in
+  make_order n;
+  bn_add_mod4 res n x y;
+  let h1 = ST.get () in
+  assert (as_nat h1 res == (as_nat h0 x + as_nat h0 y) % S.order);
+  SM.qadd_lemma (as_nat h0 x) (as_nat h0 y);
+  pop_frame ()
 
 
 val qmont_reduction: x:widefelem -> res:felem -> Stack unit
@@ -233,7 +111,7 @@ val qmont_reduction: x:widefelem -> res:felem -> Stack unit
     live h x /\ live h res /\ disjoint x res /\
     wide_as_nat h x < S.order * S.order)
   (ensures fun h0 _ h1 -> modifies (loc res |+| loc x) h0 h1 /\
-    as_nat h1 res == wide_as_nat h0 x * qmont_R_inv % S.order)
+    as_nat h1 res == wide_as_nat h0 x * SM.qmont_R_inv % S.order)
 
 [@CInline]
 let qmont_reduction x res =
@@ -248,24 +126,26 @@ let qmont_reduction x res =
   SB.bn_v_is_wide_as_nat (as_seq h0 x);
   assert (BD.bn_v (as_seq h0 n) == as_nat h0 n);
   assert (BD.bn_v (as_seq h0 x) == wide_as_nat h0 x);
-  qmont_reduction_lemma (as_seq h0 x) (as_seq h0 n);
-  assert (BD.bn_v (as_seq h1 res) == BD.bn_v (as_seq h0 x) * qmont_R_inv % S.order);
+  SM.qmont_reduction_lemma (as_seq h0 x) (as_seq h0 n);
+  assert (BD.bn_v (as_seq h1 res) == BD.bn_v (as_seq h0 x) * SM.qmont_R_inv % S.order);
   SB.bn_v_is_as_nat (as_seq h1 res);
-  assert (as_nat h1 res == wide_as_nat h0 x * qmont_R_inv % S.order);
+  assert (as_nat h1 res == wide_as_nat h0 x * SM.qmont_R_inv % S.order);
   pop_frame ()
 
-//-------------------
 
 [@CInline]
-let qadd x y res =
-  let h0 = ST.get () in
+let from_qmont a res =
   push_frame ();
-  let n = create_felem () in
-  make_order n;
-  bn_add_mod4 res n x y;
+  let t = create_widefelem () in
+  let t_low = sub t (size 0) (size 4) in
+  let t_high = sub t (size 4) (size 4) in
+
+  let h0 = ST.get () in
+  copy t_low a;
   let h1 = ST.get () in
-  assert (as_nat h1 res == (as_nat h0 x + as_nat h0 y) % S.order);
-  qadd_lemma (as_nat h0 x) (as_nat h0 y);
+  assert (wide_as_nat h0 t = as_nat h0 t_low + as_nat h0 t_high * pow2 256);
+  assert_norm (S.order < S.order * S.order);
+  qmont_reduction t res;
   pop_frame ()
 
 
@@ -278,21 +158,18 @@ let qmul a b res =
   let h1 = ST.get () in
   Math.Lemmas.lemma_mult_lt_sqr (as_nat h0 a) (as_nat h0 b) S.order;
   qmont_reduction tmp res;
-  qmul_lemma (as_nat h0 a) (as_nat h0 b);
+  SM.qmul_lemma (as_nat h0 a) (as_nat h0 b);
   pop_frame ()
 
 
 [@CInline]
-let fromDomainImpl a res =
+let qsqr a res =
   push_frame ();
-  let t = create_widefelem () in
-  let t_low = sub t (size 0) (size 4) in
-  let t_high = sub t (size 4) (size 4) in
-
+  let tmp = create_widefelem () in
   let h0 = ST.get () in
-  copy t_low a;
+  bn_sqr4 tmp a;
   let h1 = ST.get () in
-  assert (wide_as_nat h0 t = as_nat h0 t_low + as_nat h0 t_high * pow2 256);
-  assert_norm (S.order < S.order * S.order);
-  qmont_reduction t res;
+  Math.Lemmas.lemma_mult_lt_sqr (as_nat h0 a) (as_nat h0 a) S.order;
+  qmont_reduction tmp res;
+  SM.qmul_lemma (as_nat h0 a) (as_nat h0 a);
   pop_frame ()
