code/ecdsap256/Hacl.Impl.P256.Scalar.fsti
@@ -11,15 +11,22 @@ open Lib.Buffer
 open Hacl.Impl.P256.Bignum
 
 module S = Spec.P256
+module SM = Hacl.Spec.P256.Montgomery
 
 #set-options "--z3rlimit 30 --fuel 0 --ifuel 0"
 
-val qmod_short: x:felem -> res:felem -> Stack unit
-  (requires fun h ->
-    live h x /\ live h res /\ eq_or_disjoint x res)
-  (ensures fun h0 _ h1 -> modifies (loc res) h0 h1 /\
-    as_nat h1 res == as_nat h0 x % S.order)
+let qmont_as_nat (h:mem) (a:felem) = SM.fromDomain_ (as_nat h a)
 
+///  Create one
+
+val make_qone: n:felem -> Stack unit
+  (requires fun h -> live h n)
+  (ensures  fun h0 _ h1 -> modifies (loc n) h0 h1 /\
+    as_nat h1 n == SM.toDomain_ 1 /\
+    qmont_as_nat h1 n == 1)
+
+
+///  Comparison
 
 val bn_is_lt_order_mask4: f:felem -> Stack uint64
   (requires fun h -> live h f)
@@ -33,19 +40,15 @@ val bn_is_lt_order_and_gt_zero_mask4: f:felem -> Stack uint64
     (if 0 < as_nat h0 f && as_nat h0 f < S.order then v r = ones_v U64 else v r = 0))
 
 
-let qmont_R = pow2 256
-let qmont_R_inv = S.modp_inv2_prime (pow2 256) S.order
+///  Field Arithmetic
 
-// TODO: rename
-let fromDomain_ (a:nat) : S.qelem = a * qmont_R_inv % S.order
-let toDomain_   (a:nat) : S.qelem = a * qmont_R % S.order
+val qmod_short: x:felem -> res:felem -> Stack unit
+  (requires fun h ->
+    live h x /\ live h res /\ eq_or_disjoint x res)
+  (ensures fun h0 _ h1 -> modifies (loc res) h0 h1 /\
+    as_nat h1 res == as_nat h0 x % S.order)
 
-val lemmaFromDomainToDomain: a:S.qelem -> Lemma (toDomain_ (fromDomain_ a) == a)
-val lemmaToDomainFromDomain: a:S.qelem -> Lemma (fromDomain_ (toDomain_ a) == a)
 
-let qmont_as_nat (h:mem) (a:felem) = fromDomain_ (as_nat h a)
-
-// NOTE: changed precondition `eq_or_disjoint x y`
 val qadd: x:felem -> y:felem -> res:felem -> Stack unit
   (requires fun h ->
     live h x /\ live h y /\ live h res /\
@@ -56,21 +59,29 @@ val qadd: x:felem -> y:felem -> res:felem -> Stack unit
     qmont_as_nat h1 res == S.qadd (qmont_as_nat h0 x) (qmont_as_nat h0 y))
 
 
-val qmul: a:felem -> b:felem -> res:felem -> Stack unit
-  (requires fun h ->
-    live h a /\ live h b /\ live h res /\
-    eq_or_disjoint a b /\
-    as_nat h a < S.order /\ as_nat h b < S.order)
-  (ensures fun h0 _ h1 -> modifies (loc res) h0 h1 /\
-    as_nat h1 res = (as_nat h0 a * as_nat h0 b * qmont_R_inv) % S.order /\
-    qmont_as_nat h1 res = S.qmul (qmont_as_nat h0 a) (qmont_as_nat h0 b))
-
-
-// rename
-val fromDomainImpl: a:felem -> res:felem -> Stack unit
+val from_qmont: a:felem -> res:felem -> Stack unit
   (requires fun h ->
     live h a /\ live h res /\ eq_or_disjoint a res /\
     as_nat h a < S.order)
   (ensures fun h0 _ h1 -> modifies (loc res) h0 h1 /\
     as_nat h1 res < S.order /\
     as_nat h1 res == qmont_as_nat h0 a)
+
+
+val qmul: a:felem -> b:felem -> res:felem -> Stack unit
+  (requires fun h ->
+    live h a /\ live h b /\ live h res /\
+    eq_or_disjoint a b /\ eq_or_disjoint a res /\ eq_or_disjoint b res /\
+    as_nat h a < S.order /\ as_nat h b < S.order)
+  (ensures fun h0 _ h1 -> modifies (loc res) h0 h1 /\
+    as_nat h1 res = (as_nat h0 a * as_nat h0 b * SM.qmont_R_inv) % S.order /\
+    qmont_as_nat h1 res = S.qmul (qmont_as_nat h0 a) (qmont_as_nat h0 b))
+
+
+val qsqr: a:felem -> res:felem -> Stack unit
+  (requires fun h ->
+    live h a /\ live h res /\ eq_or_disjoint a res /\
+    as_nat h a < S.order)
+  (ensures fun h0 _ h1 -> modifies (loc res) h0 h1 /\
+    as_nat h1 res = (as_nat h0 a * as_nat h0 a * SM.qmont_R_inv) % S.order /\
+    qmont_as_nat h1 res = S.qmul (qmont_as_nat h0 a) (qmont_as_nat h0 a))
